add divergence + fix stuckness

theories/adequacy.v
@@ -1,24 +1,6 @@
-From stbor Require Import simulation steps_wf.
 From Paco Require Import paco.
 
-(* TODO: what about divergence and stuckness? *)
-
-Inductive behaviors
-  (step: expr * state → expr * state → Prop)
-  (cfg: expr * state) : option val → Prop :=
-| behaviors_term v
-    (TERMINAL: terminal cfg.1)
-    (EQV: sim_val_expr cfg.1 (of_val v)) :
-    behaviors step cfg (Some v)
-| behaviors_stuck
-    (NT: ¬ terminal cfg.1)
-    (NS: ∀ cfg', ¬ step cfg cfg') :
-    behaviors step cfg None
-| behaviors_step cfg' ov
-    (STEP: step cfg cfg')
-    (NEXT: behaviors step cfg' ov):
-    behaviors step cfg ov
-.
+From stbor Require Import simulation.
 
 (* If c1 ->* c2 -b-> v then c1 -b-> v *)
 Lemma rtc_step_behavior step c1 c2 v
@@ -26,36 +8,38 @@ Lemma rtc_step_behavior step c1 c2 v
   behaviors step c1 v.
 Proof.
   induction STEPS as [|c1 c2 c3 S1 S2 IH]; [done|]. specialize (IH BEH).
-  econstructor 3; eauto.
+  econstructor 4; eauto.
 Qed.
 
-Lemma sim_thread_adequacy (cfg_src cfg_tgt: expr * state)
+Lemma sim_adequacy (cfg_src cfg_tgt: expr * state)
   (WFS: Wf cfg_src.2) (WFT: Wf cfg_tgt.2)
-  (SIM: sim_thread (sim_terminal (λ _ _, True)) cfg_src cfg_tgt) :
-  ∀ ov, behaviors thread_step cfg_tgt ov → behaviors thread_step cfg_src ov.
+  (NO_UB: ∀ cfg', cfg_src ~t~>* cfg' → ¬ stuck cfg'.1 cfg'.2)
+  (SIM: sim (* (sim_terminal (λ _ _, True)) *) cfg_src cfg_tgt) :
+  behaviors tstep cfg_tgt <1= behaviors tstep cfg_src.
 Proof.
-  intros ov BEH. revert cfg_src WFS WFT SIM.
-  induction BEH as [cfg_tgt|cfg_tgt v|cfg_tgt cfg_tgt' ov STEP BEH IH];
-    intros cfg_src WFS WFT SIM.
-  - punfold SIM.
-    destruct (SIM WFS WFT) as [TERM ?].
-    destruct (TERM TERMINAL) as (eσ2 & TS & TERM' & VAL).
+  intros ov BEH. revert cfg_src WFS WFT NO_UB SIM.
+  induction BEH as [cfg_tgt|cfg_tgt|cfg_tgt v|cfg_tgt cfg_tgt' ov STEP BEH IH];
+    intros cfg_src WFS WFT NO_UB SIM.
+  - punfold SIM. destruct (SIM WFS WFT) as (? & ? & TERM & ?); [naive_solver|].
+    destruct TERM as (eσ2 & TS & TERM' & VAL); [by eexists|].
     apply (rtc_step_behavior _ _ _ _ TS).
-    constructor 1; [done|simpl]. etrans; eauto. by inversion VAL.
-  - punfold SIM.
-    destruct (SIM WFS WFT) as [TE [SU TS]].
+    constructor. by apply VAL.
+  - punfold SIM. destruct (SIM WFS WFT) as (SU & DIV & ?); [naive_solver|].
     destruct SU as [eσ2 [TS' [IN NR]]].
     + split; [by apply expr_terminal_False|].
       intros ???? PRIM. eapply (NS (e', σ')). econstructor; eauto.
     + apply (rtc_step_behavior _ _ _ _ TS').
       constructor 2; [by apply expr_terminal_False|].
       intros ? RED. inversion RED. by apply (NR _ _ _ _ PRIM).
+  - punfold SIM. destruct (SIM WFS WFT) as (SU & DIV & ?); [naive_solver|].
+    constructor. by apply DIV.
   - punfold SIM.
-    destruct (SIM WFS WFT) as [? [SU TS]].
+    destruct (SIM WFS WFT) as (SU & DIV & TERM & TS); [naive_solver|].
     destruct (TS cfg_tgt' STEP) as (eσ & STEP' & TS').
     eapply rtc_step_behavior; first by apply STEP'.
     apply IH; simpl.
-    + by apply (rtc_thread_step_wf _ _ STEP').
-    + by apply (thread_step_wf _ _ STEP).
+    + by apply (rtc_tstep_wf _ _ STEP').
+    + by apply (tstep_wf _ _ STEP).
+    + intros cfg' S'. apply NO_UB. by etrans.
     + by inversion TS'.
 Qed.
