theories/steps_inversion.v
@@ -1,5 +1,8 @@
 Require Import Coq.Program.Equality.
+
 From stbor Require Export properties steps_wf.
+
+Set Default Proof Using "Type".
 
 Ltac inv_head_step :=
   repeat match goal with
@@ -14,9 +17,9 @@ Ltac inv_head_step :=
       inversion H ; subst; clear H
   end.
 
-Ltac inv_thread_step :=
+Ltac inv_tstep :=
   repeat match goal with
-  | H : thread_step _ _ |- _ => inversion_clear H
+  | H : tstep _ _ |- _ => inversion_clear H
   | H : prim_step _ _ _ _ _ _ |- _ =>
       simpl in H; inversion_clear H as [??? Eq ? HS]; subst
   end.
@@ -41,12 +44,12 @@ Proof.
   - subst K. right. by exists v1, (Ki :: K').
 Qed.
 
-Lemma thread_step_bin_op_left_non_terminal op e1 e2 e' σ σ'
+Lemma tstep_bin_op_left_non_terminal op e1 e2 e' σ σ'
   (STEP: (BinOp op e1 e2, σ) ~t~> (e', σ'))
   (NT: ¬ terminal e1):
   ∃ e1', (e1, σ) ~t~> (e1', σ') ∧ e' = BinOp op e1' e2.
 Proof.
-  inv_thread_step.
+  inv_tstep.
   have Eq1: BinOp op e1 e2 = ectx_language.fill [BinOpLCtx op e2] e1 by done.
   rewrite Eq1 in Eq.
   apply expr_terminal_False in NT.
@@ -58,13 +61,13 @@ Proof.
   - by rewrite Eq' -fill_comp.
 Qed.
 
-Lemma thread_step_bin_op_right_non_terminal op e1 e2 e' σ σ'
+Lemma tstep_bin_op_right_non_terminal op e1 e2 e' σ σ'
   (STEP: (BinOp op e1 e2, σ) ~t~> (e', σ'))
   (TM: terminal e1) (NT: ¬ terminal e2):
   ∃ e2', (e2, σ) ~t~> (e2', σ') ∧ e' = BinOp op e1 e2'.
 Proof.
-  inv_thread_step.
-  move : TM => /expr_terminal_True [v1 Eqv1].
+  inv_tstep.
+  move : TM => [v1 Eqv1].
   have Eq1: BinOp op e1 e2 = ectx_language.fill [BinOpRCtx op v1] e2.
   { by rewrite /= -(of_to_val _ _ Eqv1). }
   rewrite Eq1 in Eq.
@@ -77,12 +80,12 @@ Proof.
   - by rewrite Eq' -fill_comp -(of_to_val _ _ Eqv1) /=.
 Qed.
 
-Lemma thread_step_bin_op_terminal op e1 e2 e' σ σ'
+Lemma tstep_bin_op_terminal op e1 e2 e' σ σ'
   (STEP: (BinOp op e1 e2, σ) ~t~> (e', σ'))
   (TM1: terminal e1) (TM2: terminal e2):
   σ' = σ ∧ ∃ l1 l2 l, bin_op_eval σ.(cheap) op l1 l2 l ∧ e' = (TVal [Lit l]).
 Proof.
-  inv_thread_step. symmetry in Eq.
+  inv_tstep. symmetry in Eq.
   destruct (fill_bin_op_decompose _ _ _ _ _ Eq)
     as [[]|[[K' [? Eq']]|[v1 [K' [? [Eq' VAL]]]]]]; subst.
   - clear Eq. simpl in HS. inv_head_step.
@@ -94,7 +97,7 @@ Proof.
     rewrite /= HS in TM2. by destruct TM2.
 Qed.
 
-Lemma thread_step_bin_op_red_r e1 σ1 e2 e2' σ2 op:
+Lemma tstep_bin_op_red_r e1 σ1 e2 e2' σ2 op:
   terminal e1 →
   (e2, σ1) ~t~>* (e2', σ2) →
   (BinOp op e1 e2, σ1) ~t~>* (BinOp op e1 e2', σ2).
@@ -104,7 +107,7 @@ Proof.
   destruct y as [e0 σ0].
   etrans; last apply IHS2; [|eauto..]. apply rtc_once.
   clear -H T1.
-  move : T1 => /expr_terminal_True [v1 Eqv1].
+  move : T1 => [v1 Eqv1].
   rewrite (_: BinOp op e1 e2 = ectx_language.fill [BinOpRCtx op v1] e2);
     last by rewrite /= -(of_to_val _ _ Eqv1).
   rewrite (_: BinOp op e1 e0 = ectx_language.fill [BinOpRCtx op v1] e0);
@@ -115,7 +118,7 @@ Proof.
   econstructor. econstructor; eauto.
 Qed.
 
-Lemma thread_step_bin_op_red_l e1 σ1 e1' σ1' e2 op:
+Lemma tstep_bin_op_red_l e1 σ1 e1' σ1' e2 op:
   (e1, σ1) ~t~>* (e1', σ1') →
   (BinOp op e1 e2, σ1) ~t~>* (BinOp op e1' e2, σ1').
 Proof.
@@ -134,14 +137,14 @@ Proof.
   econstructor. econstructor; eauto.
 Qed.
 
-Lemma thread_step_bin_op_red e1 σ1 e1' σ1' e2 e2' σ2' op:
+Lemma tstep_bin_op_red e1 σ1 e1' σ1' e2 e2' σ2' op:
   (e1, σ1) ~t~>* (e1', σ1') → terminal e1' →
   (e2, σ1') ~t~>* (e2', σ2') →
   (BinOp op e1 e2, σ1) ~t~>* (BinOp op e1' e2', σ2').
 Proof.
   intros S1 T1 S2. etrans.
-  - clear S2 T1. by eapply thread_step_bin_op_red_l.
-  - clear S1. by eapply thread_step_bin_op_red_r.
+  - clear S2 T1. by eapply tstep_bin_op_red_l.
+  - clear S1. by eapply tstep_bin_op_red_r.
 Qed.
 
 (** Copy *)
@@ -159,13 +162,13 @@ Proof.
   - subst K. by exists (Ki :: K0).
 Qed.
 
-Lemma thread_step_copy_terminal e e' σ σ'
+Lemma tstep_copy_terminal e e' σ σ'
   (STEP: (Copy e, σ) ~t~> (e', σ')) (TM: terminal e) :
   ∃ l ltag T vl , e = Place l ltag T ∧ e' = of_val (TValV vl) ∧
     read_mem l (tsize T) σ.(cheap) = Some vl
     (* not true: the stacked borrows may change, ∧ σ' = σ *).
 Proof.
-  inv_thread_step. symmetry in Eq.
+  inv_tstep. symmetry in Eq.
   destruct (fill_copy_decompose _ _ _ Eq) as [[]|[K' [? Eq']]]; subst.
   - clear Eq. simpl in HS. inv_head_step.
     (* inversion InstrStep; subst. *)
@@ -175,11 +178,11 @@ Proof.
     rewrite /= HS in TM. by destruct TM.
 Qed.
 
-Lemma thread_step_copy_non_terminal e e' σ σ'
+Lemma tstep_copy_non_terminal e e' σ σ'
   (STEP: (Copy e, σ) ~t~> (e', σ')) (NT: ¬ terminal e):
   ∃ e1, (e, σ) ~t~> (e1, σ') ∧ e' = Copy e1.
 Proof.
-  inv_thread_step.
+  inv_tstep.
   rewrite (_: Copy e = ectx_language.fill [CopyCtx] e) in Eq; [|done].
   apply expr_terminal_False in NT.
   destruct (step_by_val _ _ _ _ _ _ _ _ _ Eq NT HS) as [K'' Eq'].
